WIP: proving cancellation of main however the method should be simplified

theories/cancellation/CancelMain.v
@@ -1,27 +1,35 @@
 Require Import CRIS.
 Require Import LMod LModTr GSim GSimFacts GSimTactics.
-Require Import MInline MInlineIntro MInlineElim ElimRel.
-(* Require Import CancelCore CancelPG CancelAG CancelSpawn CancelPre CancelPost. *)
+Require Import MInline MInlineIntro MInlineElim.
+Require Import CancelCore CancelPG CancelAG CancelSpawn CancelPre CancelPost.
 
 Set Implicit Arguments.
 
 Module MainSMod. Section MainSMod.
 
-  (*** Mod to lmod modification is required : not below... ***)
-
   Context `{!crisG Γ Σ α β τ _S _I, !concG}.
+
+  Definition trans_ktree (fno: option string) sp (sb : fnsem_type (option fspec * fbody)) : fnsem_type fbody :=
+    map_snd (λ '(fsp,bd), SModTr.trans_body (is_some sb.2.1, if sb.1.1.1 then sp else sp_none, if is_some fno then fsp else None) bd) sb.
+
+  Definition map_fnsems sp (fnsems: fnsems_type) :=
+    List.map (λ '(fno, fnsem), (fno, trans_ktree fno sp fnsem)) fnsems.
+
+  Lemma alist_find_map_fnsems fn sp fnsems :
+    alist_find fn (map_fnsems sp fnsems) = o_map (alist_find fn fnsems) (λ fnsem, trans_ktree fn sp fnsem).
+  Proof.
+    rewrite /map_fnsems.
+    destruct (alist_find fn fnsems) eqn:E; ss; des_ifs; induction fnsems; ss; des_ifs; try (destruct o; ss); try (rewrite IHfnsems; ss); rewrite eq_rel_dec_correct in Heq0; des_ifs.
+  Qed.
 
   Program Definition to_mod (sp : sp_type) (ms : SMod.t) : Mod.t := {|
     Mod.scopes := ms.(SMod.scopes);
-    Mod.fnsems := List.map (λ '(fno, fnsem), (fno, SModTr.trans_ktree (if is_some fno then sp else sp_none) fnsem)) ms.(SMod.fnsems);
+    Mod.fnsems := map_fnsems sp ms.(SMod.fnsems);
     Mod.initial_st := ms.(SMod.initial_st);
     |}.
   Next Obligation.
     i. destruct ms. ss. ii. unfold fnsems_scopes in *.
-    set (m:=map _) in H0.
-    replace (alist_find fn (m fnsems)) with (o_map (alist_find fn fnsems) (λ fnsem, SModTr.trans_ktree (if fn then sp else sp_none) fnsem)) in H0; cycle 1.
-    { subst m. destruct (alist_find fn fnsems) eqn:E; ss; des_ifs; rewrite -Heq; clear -E; induction fnsems; ss; des_ifs;
-          try (by destruct o; ss); try (by rewrite IHfnsems; eauto). }
+    rewrite alist_find_map_fnsems in H0.
     specialize (well_scoped_fns fn a).
     destruct (alist_find fn fnsems) eqn: E; ss.
     destruct f. et.
@@ -41,20 +49,15 @@ Lemma cancel_main md rs
   (VALID: ✓ rs)
   :  
   refines_lmod
-    (Mod.to_lmod (MInline.inline (MainSMod.to_mod (sp_from md) md)) rs)
-    (Mod.to_lmod (MInline.inline (SMod.to_mod (sp_from md) md)) rs).
+    (Mod.to_lmod (MInline.inline false (MainSMod.to_mod (sp_from md) md)) rs)
+    (Mod.to_lmod (MInline.inline false (SMod.to_mod (sp_from md) md)) rs).
 Proof using.
   r. intro arg. eapply gsim_adequacy.
   instantiate (1:= smj_top). instantiate (1:= smj_top).
   unfold LMod.compile. s. rewrite /ITree.map /LModTr.trans /LModTr.interp_callE.  
 
   rewrite !alist_find_map_snd.
-  set (fnsems := SMod.fnsems md).
-  set (m := map _).
-  replace (alist_find None (m fnsems)) with (o_map (alist_find None fnsems) (λ fnsem, SModTr.trans_ktree sp_none fnsem)); cycle 1.
-  { subst m. destruct (alist_find None fnsems) eqn: E; ss;
-      induction fnsems; ss; des_ifs; try (destruct o; ss); try (rewrite IHfnsems; ss). }
-  subst m fnsems.
+  rewrite !MainSMod.alist_find_map_fnsems.
   destruct (alist_find None (SMod.fnsems md)) eqn: FIND; cycle 1.
   { s. ired. ginit. gstep. econs. econs. ss. }
   s. ired. rewrite /ModTr.trans_ktree.
@@ -73,7 +76,6 @@ Proof using.
 
   ziter_l. zstep_l. ziter_l. zstep_l.
   exploit WFS; et. i; des; subst; ss.
-  
   
   ginit. guclo bindC_spec. econs; cycle 1.
   { instantiate (1:=cancel_eq). i. gstep. econs. econs.
