theories/cancellation/MInlineElim.v
@@ -9,7 +9,7 @@ Set Implicit Arguments.
 Section INLINE.
 Context `{_crisG: !crisG Γ Σ α β τ _S _I}.
 
-Lemma inline_elim md P : refines (md, P) (MInline.inline md, P).
+Lemma inline_elim md P : refines (md, P) (MInline.inline false md, P).
 Proof using.
   eapply closed_adequacy_emp.
 
@@ -17,9 +17,9 @@ Proof using.
   isim_fsem
     (map (map_snd SB.sandbox_body) (Mod.fnsems md))            
     (map (map_snd SB.sandbox_body)
-       (map (map_snd (inline_fsem md)) (Mod.fnsems md)))
+       (map (map_snd (inline_fsem false md)) (Mod.fnsems md)))
      IstEq closed IstEq IstEq
-    (SB.sandbox_body f) (SB.sandbox_body (inline_fsem md f))).
+    (SB.sandbox_body f) (SB.sandbox_body (inline_fsem false md f))).
   {
     econs; ss; try refl; eauto; i.
     { i. rewrite List.map_map fst_map_snd. exists []. ss. }
@@ -42,7 +42,7 @@ Proof using.
   destruct f as [[[img msk] scp] bd].
   rewrite /SB.sandbox_body; s. rewrite /SB.sandbox_body; s.
 
-  generalize false at 1 as ps. generalize false at 1 as pt.
+  generalize false at 2 as ps. generalize false at 2 as pt.
   generalize (bd arg) as it. i.
   ss. clear bd arg. rename st_tgt into st.
 
@@ -88,7 +88,7 @@ Proof using.
         ii. exploit Mod.well_scoped_fns; et.
         rewrite /fnsems_scopes. erewrite FIND. et.
       - iIntros (? ? ? ?) "%". des; subst.
-        rewrite MIRed.tau. steps_l. steps_r. ired.
+        rewrite !bind_tau !bind_ret_l !MIRed.tau. steps_l. steps_r. ired.
         by_coind CIH; et.
     }
     {
